refactoring

src/multiplier.v
@@ -26,9 +26,15 @@
 (*                                                                                *)
 (**********************************************************************************)
 
-From stdpp Require Import base tactics decidable.
-From research Require Import bitvector.
+From stdpp Require Import base tactics bitvector.
 From RecordUpdate Require Import RecordUpdate.
+
+Local Open Scope bv_scope.
+
+Ltac Zify.zify_post_hook ::= Z.div_mod_to_equations.
+
+Ltac simplify :=
+  repeat progress (intros; csimpl in *; subst).
 
 Definition make_visible {X} (f : X) := f.
 
@@ -37,327 +43,303 @@ Notation "` f" := (make_visible f) (at level 10, format "` f").
 Tactic Notation "unfold" "notation" constr(f) := change f with (`f).
 Tactic Notation "fold" "notation" constr(f) := unfold make_visible.
 
-Section Common.
-  Record Registers :=
-    mkRegisters
-      { RA : bv 8
-      ; RB : bv 4
-      ; RCount : bv 2
-      ; RBusy : bv 1
-      }.
+Definition bv_eqb {n} (x y : bv n) : bool :=
+  Eval cbv beta iota zeta delta [ bool_decide decide_rel ] in
+    bool_decide (x = y).
 
-  Definition Registers0 := mkRegisters 0 0 0 0.
+Definition bv_odd {n} (x : bv n) := Z.odd (bv_unsigned x).
 
-  Record In :=
-    mkIn
-      { InA : bv 4
-      ; InB : bv 4
-      ; InValid : bv 1
-      }.
+Infix "=?" := bv_eqb : bv_scope.
+Infix "#" := bv_zero_extend (at level 65) : bv_scope.
+Infix "||" := (bv_concat _) : bv_scope.
 
-  Definition In0 := mkIn 0 0 0.
+Record Registers := mkRegisters { RA : bv 8 ; RB : bv 4 ; RCount : bv 2 ; RBusy : bv 1}.
 
-  Record Out :=
-    mkOut
-      { OutP : bv 8
-      ; OutReady : bv 1 }.
+Definition Registers0 := mkRegisters 0 0 0 0.
 
-  Definition Out0 := mkOut 0 0.
-End Common.
+Record In := mkIn { InA : bv 4 ; InB : bv 4 ; InValid : bv 1}.
 
-Module Circuit1.
-  Local Open Scope bv_scope.
+Definition In0 := mkIn 0 0 0.
 
-  Record ILeakage :=
-    mkILeak
-      { LeakValid : bv 1
-      ; LeakReady : bv 1
-      }.
+Record Out := mkOut { OutP : bv 8 ; OutReady : bv 1 }.
 
-  Record State :=
-    mkState
-      { R : Registers
-      ; T : list ILeakage
-      }.
+Definition Out0 := mkOut 0 0.
 
-  Definition State0 := mkState Registers0 [].
+Record ILeakage := mkILeak { LeakValid : bv 1 ; LeakReady : bv 1}.
 
-  (* One shift-and-add step: conditionally add `b` into the high half of `a`
-     then shift-right by one by reassembly. *)
-  Definition shift_and_add (b : bv 4) (a : bv 8) : bv 8 :=
-    let t0 := bv_extract 4 5 a in
-    let t1 := if bv_odd a then 5#b else 0 in
-    (t0 + t1) || (bv_extract 1 3 a).
+Record State := mkState { R : Registers ; T : list ILeakage}.
 
-  Definition cycle (s : State) (x : In) : State * Out :=
-    if s.(R).(RBusy) =? 0
+Definition State0 := mkState Registers0 [].
+
+(* One shift-and-add step: conditionally add `b` into the high half of `a` then
+   shift-right by one by reassembly. *)
+Definition shift_and_add (b : bv 4) (a : bv 8) : bv 8 :=
+  let t0 := bv_extract 4 5 a in
+  let t1 := if bv_odd a then 5#b else 0 in
+  t0 + t1 || bv_extract 1 3 a.
+
+Definition cycle (s : State) (x : In) : State * Out :=
+  if s.(R).(RBusy) =? 0
+  then
+    if x.(InValid) =? 1
     then
-      if x.(InValid) =? 1
-      then
-        let ra' := 8#x.(InA) in
-        let rb' := x.(InB) in
-        let rcount' := 3 in
-        let rbusy' := 1 in
-        let r' := mkRegisters ra' rb' rcount' rbusy' in
-        let t' := s.(T) ++ [mkILeak x.(InValid) 0 ] in
-        let s' := mkState r' t' in
-        (s', Out0)
-      else
-        let t' := s.(T) ++ [mkILeak x.(InValid) 0 ] in
-        let r' := s.(R) in
-        let s' := mkState r' t' in
-        (s', Out0)
+      let ra' := 8#x.(InA) in
+      let rb' := x.(InB) in
+      let rcount' := 3 in
+      let rbusy' := 1 in
+      let r' := mkRegisters ra' rb' rcount' rbusy' in
+      let t' := s.(T) ++ [mkILeak x.(InValid) 0 ] in
+      let s' := mkState r' t' in
+      (s', Out0)
     else
-      let ra' := shift_and_add s.(R).(RB) s.(R).(RA) in
-      let rb' := s.(R).(RB) in
-      if s.(R).(RCount) =? 0
-      then
-        let rcount' := 0 in
-        let rbusy' := 0 in
-        let r' := mkRegisters ra' rb' rcount' rbusy' in
-        let t' := s.(T) ++ [mkILeak x.(InValid) 1 ] in
-        let s' := mkState r' t' in
-        let o' := mkOut ra' 1 in
-        (s', o')
-      else
-        let rcount' := s.(R).(RCount) - 1 in
-        let rbusy' := 1 in
-        let r' := mkRegisters ra' rb' rcount' rbusy' in
-        let t' := s.(T) ++ [mkILeak x.(InValid) 0 ] in
-        let s' := mkState r' t' in
-        (s', Out0).
+      let t' := s.(T) ++ [mkILeak x.(InValid) 0 ] in
+      let r' := s.(R) in
+      let s' := mkState r' t' in
+      (s', Out0)
+  else
+    let ra' := shift_and_add s.(R).(RB) s.(R).(RA) in
+    let rb' := s.(R).(RB) in
+    if s.(R).(RCount) =? 0
+    then
+      let rcount' := 0 in
+      let rbusy' := 0 in
+      let r' := mkRegisters ra' rb' rcount' rbusy' in
+      let t' := s.(T) ++ [mkILeak x.(InValid) 1 ] in
+      let s' := mkState r' t' in
+      let o' := mkOut ra' 1 in
+      (s', o')
+    else
+      let rcount' := s.(R).(RCount) - 1 in
+      let rbusy' := 1 in
+      let r' := mkRegisters ra' rb' rcount' rbusy' in
+      let t' := s.(T) ++ [mkILeak x.(InValid) 0 ] in
+      let s' := mkState r' t' in
+      (s', Out0).
 
-  Fixpoint cycles (s : State) (xs : list In) : State * list Out :=
-    match xs with
-    | [] => (s, [])
-    | x :: xs' =>
-        let (s', y) := cycle s x in
-        let (s'', ys) := cycles s' xs' in
-        (s'', y :: ys)
+Fixpoint cycles (s : State) (xs : list In) : State * list Out :=
+  match xs with
+  | [] => (s, [])
+  | x :: xs' =>
+      let (s', y) := cycle s x in
+      let (s'', ys) := cycles s' xs' in
+      (s'', y :: ys)
+  end.
+
+Fixpoint repeat {A : Type} (f : A -> A) (n : nat) {struct n} : (A -> A) :=
+  match n with
+  | O => id
+  | S n' => f ∘ repeat f n'
+  end.
+
+Definition repeat_shift_and_add n b a := (repeat (shift_and_add b) n) a.
+
+Definition shift_and_add4 := repeat_shift_and_add 4.
+
+Definition shift_and_add' (b a : Z) :=
+  Z.lor (bv_wrap 5 (a ≫ 4 + (bv_wrap 1 a * b)) ≪ 3) (bv_wrap 3 (a ≫ 1)).
+
+Definition repeat_shift_and_add' n b a := (repeat (shift_and_add' b) n) a.
+
+Definition shift_and_add4' := repeat_shift_and_add' 4.
+
+Lemma shift_and_add_equiv : forall a b,
+    shift_and_add' (bv_unsigned b) (bv_unsigned a) =
+      bv_unsigned (shift_and_add b a).
+Proof.
+  intros a b. unfold shift_and_add, shift_and_add'. bv_simplify.
+  unfold Z.of_N, bv_odd. unfold notation Z.modulo. Search (_ `mod` 2)%Z.
+  unfold bv_wrap. rewrite Zmod_odd. case_match.
+  - replace (1 * bv_unsigned b)%Z with (bv_unsigned b) by lia. bv_solve.
+  - Search (0 * _)%Z. rewrite Z.mul_0_l. bv_solve.
+Qed.
+
+Lemma shift_and_add_repeat_equiv : forall n a b,
+    (repeat_shift_and_add' n) (bv_unsigned b) (bv_unsigned a) =
+      bv_unsigned (repeat_shift_and_add n b a).
+Proof.
+  intros n a b. induction n; simplify.
+  - unfold repeat_shift_and_add', repeat_shift_and_add. done.
+  - unfold repeat_shift_and_add', repeat_shift_and_add in *. simplify.
+    rewrite IHn. apply shift_and_add_equiv.
+Qed.
+
+Lemma shift_and_add4_equiv : forall a b,
+    shift_and_add4' (bv_unsigned b) (bv_unsigned a) =
+      bv_unsigned (shift_and_add4 b a).
+Proof.
+  unfold shift_and_add4', shift_and_add4. apply shift_and_add_repeat_equiv.
+Qed.
+
+(* Tactic for exhaustive case analysis on integers in range [0,16) *)
+(* Automatically finds variables with range hypotheses and does case analysis *)
+Ltac case_range16 :=
+  repeat match goal with
+    | [ H : (0 <= ?z < 16)%Z |- _ ] =>
+        let Hz := fresh "Hcases" in
+        assert (z = 0 \/ z = 1 \/ z = 2 \/ z = 3 \/ z = 4 \/ z = 5 \/ z = 6 \/ z = 7 \/
+                  z = 8 \/ z = 9 \/ z = 10 \/ z = 11 \/ z = 12 \/ z = 13 \/ z = 14 \/ z = 15)%Z
+          as Hz by lia; clear H;
+        destruct_or?; subst
+    end; done.
+
+Lemma shift_and_add4'_multiplies : forall a b,
+    (0 <= a < bv_modulus 4%N)%Z ->
+    (0 <= b < bv_modulus 4%N)%Z ->
+    shift_and_add4' b a = (a * b)%Z.
+Proof.
+  intros a b Ha Hb.
+  replace (bv_modulus 4%N) with 16%Z in * by trivial.
+  rewrite Z.mul_comm.
+  case_range16.
+Qed.
+
+Lemma shift_and_add4_multiplies : forall (a b : bv 4),
+    bv_unsigned (shift_and_add4 b (8#a)) = (bv_unsigned a * bv_unsigned b)%Z.
+Proof.
+  intros a b. rewrite <- shift_and_add4_equiv.
+  Search bv_unsigned bv_zero_extend. rewrite bv_zero_extend_unsigned by lia.
+  apply shift_and_add4'_multiplies. all: bv_solve.
+Qed.
+
+Notation "a *| b" := ((8#a) * (8#b)) (at level 35).
+
+Lemma shift_and_add4_correct : forall (a b : bv 4),
+    shift_and_add4 b (8#a) = a *| b.
+Proof.
+  intros a b. Search (bv_unsigned _ = bv_unsigned _).
+  rewrite bv_eq. Search bv_mul.
+  rewrite bv_mul_unsigned.
+  Search bv_zero_extend bv_unsigned.
+  repeat rewrite bv_zero_extend_unsigned by lia.
+  Check bv_wrap_small. rewrite bv_wrap_small.
+  apply shift_and_add4_multiplies. bv_saturate_unsigned.
+  unfold bv_modulus in *; simplify. nia.
+Qed.
+
+Lemma bv1_is_0_or_1 : forall (b : bv 1), b = 0 \/ b = 1.
+Proof.
+  intro b. Search "bv" "ind".
+  apply bv_1_ind with (P := (fun b => b = 0 \/ b = 1)); intuition congruence.
+Qed.
+
+Definition busy (s : State) := s.(R).(RBusy) = 1.
+Definition finished (s : State) := s.(R).(RCount) = 0.
+Definition valid (x : In) := x.(InValid) = 1.
+
+Hint Extern 1 (_ = _ :> bv 1) =>
+       match goal with
+       | |- ?b = 0 :> bv 1 => pose proof (bv1_is_0_or_1 b); intuition
+| |- ?b = 1 :> bv 1 => pose proof (bv1_is_0_or_1 b); intuition
+end : multiplier.
+
+Definition cycle_idle_valid s1 x s2 y : Prop :=
+  ~ busy s1 -> valid x -> (s2, y) = cycle s1 x ->
+  (s2, y) = (s1 <| R := {| RA := 8#x.(InA); RB := x.(InB); RCount := 3; RBusy := 1 |} |>
+                <| T := s1.(T) ++ [{| LeakValid := 1; LeakReady := 0 |}] |>,
+             Out0).
+
+Lemma cycle_idle_valid_holds : forall s1 x s2 y, cycle_idle_valid s1 x s2 y.
+Proof.
+  unfold cycle_idle_valid. simplify.
+  unfold cycle in *. unfold bv_eqb in *. unfold busy in *.
+  unfold valid in *. assert (s1.(R).(RBusy) = 0) by auto with multiplier.
+  repeat rewrite H2 in H1. simpl in *. rewrite H0 in H1.
+  simplify. inv H1. done.
+Qed.
+
+Definition cycle_idle_invalid s1 x s2 y : Prop :=
+  ~ busy s1 -> ~ valid x -> (s2, y) = cycle s1 x ->
+  (s2, y) = (s1 <| T := s1.(T) ++ [{| LeakValid := 0; LeakReady := 0 |}] |>,
+                             Out0).
+
+Lemma cycle_idle_invalid_holds : forall s1 x s2 y, cycle_idle_invalid s1 x s2 y.
+Proof.
+  unfold cycle_idle_invalid. simplify.
+  unfold cycle, bv_eqb, busy, valid in *.
+  assert (s1.(R).(RBusy) = 0) by auto with multiplier.
+  assert (x.(InValid) = 0) by auto with multiplier.
+  rewrite H2, H3 in H1. simpl in *. inversion H1; clear H1.
+  done.
+Qed.
+
+Definition cycle_busy_unfinished s1 x s2 y : Prop :=
+  busy s1 -> ~ finished s1 -> (s2, y) = cycle s1 x ->
+  (s2, y) = (s1 <| R; RA := shift_and_add s1.(R).(RB) s1.(R).(RA) |>
+                <| R; RCount := s1.(R).(RCount) - 1 |>
+                <| T := s1.(T) ++ [{| LeakValid := x.(InValid); LeakReady := 0 |}] |>,
+              Out0).
+
+Lemma cycle_busy_unfinished_holds : forall s1 x s2 y, cycle_busy_unfinished s1 x s2 y.
+Proof.
+  unfold cycle_busy_unfinished. simplify.
+  unfold cycle, bv_eqb, busy, finished in *.
+  rewrite H in H1; simpl in *.
+  destruct (bv_eq_dec 2 (RCount (R s1)) 0) as [Heq | Hneq].
+  - done.
+  - inversion H1; clear H1; subst. intuition congruence.
+Qed.
+
+Definition cycle_busy_finished s1 x s2 y : Prop :=
+  busy s1 -> finished s1 -> (s2, y) = cycle s1 x ->
+  (s2, y) = (s1 <| R; RA := shift_and_add s1.(R).(RB) s1.(R).(RA) |>
+                <| R; RCount := 0 |>
+                <| R; RBusy := 0 |>
+                <| T := s1.(T) ++ [{| LeakValid := x.(InValid); LeakReady := 1 |}] |>,
+                {| OutP := s2.(R).(RA); OutReady := 1 |}).
+
+Lemma cycle_busy_finished_holds : forall s1 x s2 y, cycle_busy_finished s1 x s2 y.
+Proof.
+  unfold cycle_busy_finished. simplify.
+  unfold cycle, bv_eqb, busy, finished in *.
+  rewrite H in H1; simplify. rewrite H0 in H1.
+  simplify. inversion H1; clear H1; subst. done.
+Qed.
+
+Ltac unfold_cycle_predicates :=
+  unfold cycle_idle_valid, cycle_idle_invalid, cycle_busy_unfinished,
+    cycle_busy_finished, busy, finished, valid in *.
+
+Ltac unfold_pair H := inversion H; clear H.
+
+Ltac unfold_pairs :=
+  repeat match goal with
+    | H : (_, _) = (_, _) |- _ => unfold_pair H
     end.
 
-  Fixpoint repeat {A : Type} (f : A -> A) (n : nat) {struct n} : (A -> A) :=
-    match n with
-    | O => id
-    | S n' => f ∘ repeat f n'
+Ltac unroll_let e :=
+  let Hlet := fresh "Hlet0" in destruct e eqn:Hlet; symmetry in Hlet.
+
+Ltac unroll_lets :=
+  repeat match goal with
+    | [ H : context[let (_, _) := (cycle ?x ?y) in _] |- _ ] =>
+        unroll_let (cycle x y)
     end.
 
-  Definition repeat_shift_and_add n b a := (repeat (shift_and_add b) n) a.
+Ltac cycles_correct_auto :=
+  unfold_pairs; subst; try (unfold_cycle_predicates; solve
+                        [ intuition
+                        | simplify; bv_solve ]).
 
-  Definition shift_and_add4 := repeat_shift_and_add 4.
-
-  Definition shift_and_add' (b a : Z) :=
-    Z.lor (bv_wrap 5 (a ≫ 4 + (bv_wrap 1 a * b)) ≪ 3) (bv_wrap 3 (a ≫ 1)).
-
-  Definition repeat_shift_and_add' n b a := (repeat (shift_and_add' b) n) a.
-
-  Definition shift_and_add4' := repeat_shift_and_add' 4.
-
-  Lemma shift_and_add_equiv : forall a b,
-      shift_and_add' (bv_unsigned b) (bv_unsigned a) =
-        bv_unsigned (shift_and_add b a).
-  Proof.
-    intros a b. unfold shift_and_add, shift_and_add'. bv_simplify.
-    unfold Z.of_N, bv_odd. unfold notation Z.modulo. Search (_ `mod` 2)%Z.
-    unfold bv_wrap. rewrite Zmod_odd. case_match.
-    - replace (1 * bv_unsigned b)%Z with (bv_unsigned b) by lia. bv_solve.
-    - Search (0 * _)%Z. rewrite Z.mul_0_l. bv_solve.
-  Qed.
-
-  Lemma shift_and_add_repeat_equiv : forall n a b,
-      (repeat_shift_and_add' n) (bv_unsigned b) (bv_unsigned a) =
-        bv_unsigned (repeat_shift_and_add n b a).
-  Proof.
-    intros n a b. induction n; simpl.
-    - unfold repeat_shift_and_add', repeat_shift_and_add. done.
-    - unfold repeat_shift_and_add', repeat_shift_and_add in *. simpl.
-      rewrite IHn. apply shift_and_add_equiv.
-  Qed.
-
-  Lemma shift_and_add4_equiv : forall a b,
-      shift_and_add4' (bv_unsigned b) (bv_unsigned a) =
-        bv_unsigned (shift_and_add4 b a).
-  Proof.
-    unfold shift_and_add4', shift_and_add4. apply shift_and_add_repeat_equiv.
-  Qed.
-
-  (* Tactic for exhaustive case analysis on integers in range [0,16) *)
-  (* Automatically finds variables with range hypotheses and does case analysis *)
-  Ltac case_range16 :=
-    repeat match goal with
-      | [ H : (0 <= ?z < 16)%Z |- _ ] =>
-          let Hz := fresh "Hcases" in
-          assert (z = 0 \/ z = 1 \/ z = 2 \/ z = 3 \/ z = 4 \/ z = 5 \/ z = 6 \/ z = 7 \/
-                    z = 8 \/ z = 9 \/ z = 10 \/ z = 11 \/ z = 12 \/ z = 13 \/ z = 14 \/ z = 15)%Z
-            as Hz by lia; clear H;
-          destruct_or?; subst
-      end; done.
-
-  Lemma shift_and_add4'_multiplies : forall a b,
-      (0 <= a < bv_modulus 4%N)%Z ->
-      (0 <= b < bv_modulus 4%N)%Z ->
-      shift_and_add4' b a = (a * b)%Z.
-  Proof.
-    intros a b Ha Hb.
-    replace (bv_modulus 4%N) with 16%Z in * by trivial.
-    rewrite Z.mul_comm.
-    case_range16.
-  Qed.
-
-  Lemma shift_and_add4_multiplies : forall (a b : bv 4),
-      bv_unsigned (shift_and_add4 b (8#a)) = (bv_unsigned a * bv_unsigned b)%Z.
-  Proof.
-    intros a b. rewrite <- shift_and_add4_equiv.
-    Search bv_unsigned bv_zero_extend. rewrite bv_zero_extend_unsigned by lia.
-    apply shift_and_add4'_multiplies. all: bv_solve.
-  Qed.
-
-  Notation "a *| b" := ((8#a) * (8#b)) (at level 35).
-
-  Lemma shift_and_add4_correct : forall (a b : bv 4),
-      shift_and_add4 b (8#a) = a *| b.
-  Proof.
-    intros a b. Search (bv_unsigned _ = bv_unsigned _).
-    rewrite bv_eq. Search bv_mul.
-    rewrite bv_mul_unsigned.
-    Search bv_zero_extend bv_unsigned.
-    repeat rewrite bv_zero_extend_unsigned by lia.
-    Check bv_wrap_small. rewrite bv_wrap_small.
-    apply shift_and_add4_multiplies. bv_saturate_unsigned.
-    unfold bv_modulus in *; simpl in *. nia.
-  Qed.
-
-  Lemma bv1_is_0_or_1 : forall (b : bv 1), b = 0 \/ b = 1.
-  Proof.
-    intro b. Search "bv" "ind".
-    apply bv_1_ind with (P := (fun b => b = 0 \/ b = 1)); intuition congruence.
-  Qed.
-
-  Definition busy (s : State) := s.(R).(RBusy) = 1.
-  Definition finished (s : State) := s.(R).(RCount) = 0.
-  Definition valid (x : In) := x.(InValid) = 1.
-
-  Hint Extern 1 (_ = _ :> bv 1) =>
-         match goal with
-         | |- ?b = 0 :> bv 1 => pose proof (bv1_is_0_or_1 b); intuition
-         | |- ?b = 1 :> bv 1 => pose proof (bv1_is_0_or_1 b); intuition
-         end : multiplier.
-
-  Definition cycle_idle_valid s1 x s2 y : Prop :=
-      ~ busy s1 -> valid x -> (s2, y) = cycle s1 x ->
-      (s2, y) = (s1 <| R := {| RA := 8#x.(InA); RB := x.(InB); RCount := 3; RBusy := 1 |} |>
-                    <| T := s1.(T) ++ [{| LeakValid := 1; LeakReady := 0 |}] |>,
-                 Out0).
-
-  Lemma cycle_idle_valid_holds : forall s1 x s2 y, cycle_idle_valid s1 x s2 y.
-  Proof.
-    unfold cycle_idle_valid.
-    repeat progress (intros; simpl; subst).
-    unfold cycle in *. unfold bv_eqb in *. unfold busy in *.
-    unfold valid in *. assert (s1.(R).(RBusy) = 0) by auto with multiplier.
-    repeat rewrite H2 in H1. simpl in *. rewrite H0 in H1.
-    csimpl in *. inv H1. done.
-  Qed.
-
-  Definition cycle_idle_invalid s1 x s2 y : Prop :=
-    ~ busy s1 -> ~ valid x -> (s2, y) = cycle s1 x ->
-    (s2, y) = (s1 <| T := s1.(T) ++ [{| LeakValid := 0; LeakReady := 0 |}] |>,
-               Out0).
-
-  Lemma cycle_idle_invalid_holds : forall s1 x s2 y, cycle_idle_invalid s1 x s2 y.
-  Proof.
-    unfold cycle_idle_invalid.
-    repeat progress (intros; simpl; subst).
-    unfold cycle, bv_eqb, busy, valid in *.
-    assert (s1.(R).(RBusy) = 0) by auto with multiplier.
-    assert (x.(InValid) = 0) by auto with multiplier.
-    rewrite H2, H3 in H1. simpl in *. inversion H1; clear H1.
-    done.
-  Qed.
-
-  Definition cycle_busy_unfinished s1 x s2 y : Prop :=
-    busy s1 -> ~ finished s1 -> (s2, y) = cycle s1 x ->
-      (s2, y) = (s1 <| R; RA := shift_and_add s1.(R).(RB) s1.(R).(RA) |>
-                    <| R; RCount := s1.(R).(RCount) - 1 |>
-                   <| T := s1.(T) ++ [{| LeakValid := x.(InValid); LeakReady := 0 |}] |>,
-                 Out0).
-
-  Lemma cycle_busy_unfinished_holds : forall s1 x s2 y, cycle_busy_unfinished s1 x s2 y.
-  Proof.
-    unfold cycle_busy_unfinished.
-    repeat progress (intros; simpl; subst).
-    unfold cycle, bv_eqb, busy, finished in *.
-    rewrite H in H1; simpl in *.
-    destruct (bv_eq_dec 2 (RCount (R s1)) 0) as [Heq | Hneq].
-    - done.
-    - inversion H1; clear H1; subst. intuition congruence.
-  Qed.
-
-  Definition cycle_busy_finished s1 x s2 y : Prop :=
-    busy s1 -> finished s1 -> (s2, y) = cycle s1 x ->
-      (s2, y) = (s1 <| R; RA := shift_and_add s1.(R).(RB) s1.(R).(RA) |>
-                    <| R; RCount := 0 |>
-                    <| R; RBusy := 0 |>
-                    <| T := s1.(T) ++ [{| LeakValid := x.(InValid); LeakReady := 1 |}] |>,
-                 {| OutP := s2.(R).(RA); OutReady := 1 |}).
-
-  Lemma cycle_busy_finished_holds : forall s1 x s2 y, cycle_busy_finished s1 x s2 y.
-  Proof.
-    unfold cycle_busy_finished.
-    repeat progress (intros; simpl; subst).
-    unfold cycle, bv_eqb, busy, finished in *.
-    rewrite H in H1; simpl in *. rewrite H0 in H1.
-    simpl in *. inversion H1; clear H1; subst. done.
-  Qed.
-
-  Ltac simplify :=
-    repeat progress (intros; csimpl in *; subst).
-
-  Ltac unfold_cycle_predicates :=
-    unfold cycle_idle_valid, cycle_idle_invalid, cycle_busy_unfinished,
-      cycle_busy_finished, busy, finished, valid in *.
-
-  Ltac unfold_pair H := inversion H; clear H.
-
-  Ltac unfold_pairs :=
-    repeat match goal with
-      | H : (_, _) = (_, _) |- _ => unfold_pair H
-      end.
-
-  Ltac unroll_let e :=
-    let Hlet := fresh "Hlet0" in destruct e eqn:Hlet; symmetry in Hlet.
-
-  Ltac unroll_lets :=
-    repeat match goal with
-      | [ H : context[let (_, _) := (cycle ?x ?y) in _] |- _ ] =>
-          unroll_let (cycle x y)
-      end.
-
-  Ltac cauto :=
-    unfold_pairs; subst;
-    try (unfold_cycle_predicates;
-         solve [ naive_solver | csimpl in *; bv_solve ]).
-
-  (* Finally, with all those helper theorems out of the way, we can now prove
+(* Finally, with all those helper theorems out of the way, we can now prove
      the following correctness property:
 
      For any cycle where the circuit is idle, if a valid [a] and [b] are
      provided, four cycles later it will produce [a *| b]. *)
-  Theorem cycles_correct : forall s s' x1 x2 x3 x4 x5 ys a b,
-      ~ busy s -> x1 = {| InA := a; InB := b; InValid := 1 |} ->
-      (s', ys) = cycles s [x1; x2; x3; x4; x5] ->
-      ys = [Out0; Out0; Out0; Out0; {| OutP := a *| b; OutReady := 1 |}].
-  Proof.
-    simplify. unroll_lets.
-    apply cycle_idle_valid_holds in Hlet0; cauto.
-    apply cycle_busy_unfinished_holds in Hlet1; cauto.
-    apply cycle_busy_unfinished_holds in Hlet2; cauto.
-    apply cycle_busy_unfinished_holds in Hlet3; cauto.
-    apply cycle_busy_finished_holds in Hlet4; cauto.
-    simplify. repeat f_equal. by apply shift_and_add4_correct.
-  Qed.
+Theorem cycles_correct : forall s s' x1 x2 x3 x4 x5 ys a b,
+    ~ busy s -> x1 = {| InA := a; InB := b; InValid := 1 |} ->
+    (s', ys) = cycles s [x1; x2; x3; x4; x5] ->
+    ys = [Out0; Out0; Out0; Out0; {| OutP := a *| b; OutReady := 1 |}].
+Proof.
+  simplify. unroll_lets.
+  apply cycle_idle_valid_holds      in Hlet0; cycles_correct_auto.
+  apply cycle_busy_unfinished_holds in Hlet1; cycles_correct_auto.
+  apply cycle_busy_unfinished_holds in Hlet2; cycles_correct_auto.
+  apply cycle_busy_unfinished_holds in Hlet3; cycles_correct_auto.
+  apply cycle_busy_finished_holds   in Hlet4; cycles_correct_auto.
+  simplify. repeat f_equal. by apply shift_and_add4_correct.
+Qed.
 
-  (** NOTE knwabueze for aerbsen: I think we talked about using this definition
+(** NOTE knwabueze for aerbsen: I think we talked about using this definition
       for the extraction from the list of inputs to the specification leakage.
 
     {[
@@ -371,13 +353,12 @@ Module Circuit1.
     function would need to know whether or not a value for [A] was provided on
     each cycle, not just the total list of provided values. *)
 
-  Definition SLeakage := option (bv 4).
+Definition SLeakage := option (bv 4).
 
-  Definition extract : list In -> list SLeakage :=
-    map (fun x => if x.(InValid) =? 1 then Some x.(InA) else None).
+Definition extract : list In -> list SLeakage :=
+  map (fun x => if x.(InValid) =? 1 then Some x.(InA) else None).
 
-  Theorem cycles_ct : exists (predictor : list SLeakage -> list ILeakage),
-    forall (xs : list In) (ys : list Out) (s : State),
-      (s, ys) = cycles State0 xs -> s.(T) = (predictor ∘ extract) xs.
-  Admitted.
-End Circuit1.
+Theorem cycles_ct : exists (predictor : list SLeakage -> list ILeakage),
+  forall (xs : list In) (ys : list Out) (s : State),
+    (s, ys) = cycles State0 xs -> s.(T) = (predictor ∘ extract) xs.
+Admitted.
